README.md
@@ -9,7 +9,7 @@ git clone https://github.com/KiJeong-Lim/DschingisKhan.git
 cd DschingisKhan
 eval `opam env`
 coq_makefile -f _CoqProject -o Makefile
-make
+make -j2 -k
 ```
 
 ## COMPATIBLE COQ VERSIONS
